Monad_Play Around/State_Monad_HL.thy
@@ -4,12 +4,14 @@ imports
   "~~/src/HOL/Library/State_Monad"
 begin
 
+text\<open>\<close>
 definition TT:: "'a \<Rightarrow> bool" where "TT x = True"
 definition TTT:: "'b \<Rightarrow> 'a \<Rightarrow> bool" where "TTT x y = True"
 definition FF:: "'a \<Rightarrow> bool" where "FF x = False"
 definition GG:: "('a \<Rightarrow> bool) \<Rightarrow> ('b => 'a \<Rightarrow> bool)" where "GG p x = p"
 definition UU:: "('a \<Rightarrow> bool) \<Rightarrow> (unit => 'a \<Rightarrow> bool)" where "UU p x = p"
 
+section\<open>Methods to get interact with the state-monad\<close>
 definition return:: "'a \<Rightarrow> ('b, 'a) state" where "return = State_Monad.return"
 definition get_state:: "('a, 'a) state" where "get_state = State (\<lambda>x. (x,x))"
 definition put_state:: "'a \<Rightarrow> ('a, unit) state" where "put_state x = State (\<lambda>_. ((),x))"
@@ -26,9 +28,11 @@ definition assign:: "('a \<Rightarrow> 'b \<Rightarrow> 'a) \<Rightarrow> ('a \<
 definition spec:: "('a \<Rightarrow> bool) \<Rightarrow> ('a, 'b) state \<Rightarrow> ('b \<Rightarrow> 'a \<Rightarrow> bool) \<Rightarrow> bool" where 
   "spec p S q = (\<forall>x. p x  \<longrightarrow> (let (y, z) = run_state S x in q y z))"
 
+section\<open>Rules based on \<close>
 theorem get_state_rule: "spec (\<lambda>x. p x x) (get_state) p"
   by (simp add: get_state_def spec_def)
 
+text\<open>Rule to extract a value from the Monad\<close>
 theorem get_rule: "\<forall>x. spec (\<lambda>y. p y \<and> v x = v y) (S (v x)) q \<Longrightarrow> spec p (get v \<bind> S) q"
   by (simp add: spec_def get_def return_def case_prod_unfold get_state_def)
 
@@ -38,28 +42,35 @@ theorem return_rule: "spec (p v) (return v) p"
 theorem seq_rule: "\<lbrakk>spec p S q; \<forall>x. spec (q x) T r\<rbrakk> \<Longrightarrow> spec p (do { S; T }) r"
   apply (simp add: spec_def)
   by fastforce
-  
+
+text\<open>Rule to capture scope of local variables\<close>
 theorem let_rule: "let v = E in spec p (do { T }) r \<Longrightarrow> spec p (do { let v = E; T }) r"
   by (simp add: spec_def snd_def)
 
+text\<open>A skip-statement can be ignored\<close>
 theorem skip_left_rule: "spec p (do { skip; S }) q \<Longrightarrow> spec p S q"
   by (simp add: spec_def skip_def)
 
+text\<open>Pre- and post-conditions can be conjoined\<close>
 theorem conj_rule: "\<lbrakk>spec p S q; spec r S s\<rbrakk> \<Longrightarrow> spec (\<lambda>x. p x \<and> r x) S (\<lambda>x y. q x y \<and> s x y)"
   apply (simp add: spec_def)
   by (simp add: case_prod_unfold)
 
+text\<open>A conjunction of the post-condition can be split up and be proved separately\<close>
 theorem conj_rule_right: "\<lbrakk>spec p S q; spec p S s\<rbrakk> \<Longrightarrow> spec p S (\<lambda>x y. q x y \<and> s x y)"
   apply (simp add: spec_def)
   by (simp add: case_prod_unfold)
 
+text\<open>A pre-condition be weaken if it still preserves the post-condition (Weakest pre-condition)\<close>
 theorem weaken_rule: "\<lbrakk>\<forall>x. (p x \<longrightarrow> p0 x); spec p0 S q\<rbrakk> \<Longrightarrow> spec p S q"
   by (simp add: spec_def)
 
+text\<open>A post-condition can be strengthen if it gets preserved by the pre-condition\<close>
 theorem strengthen_rule: "\<lbrakk>\<forall>x y. (q0 x y \<longrightarrow> q x y); spec p S q0\<rbrakk> \<Longrightarrow> spec p S q"
   apply (simp add: spec_def)
   by (simp add: case_prod_unfold)
 
+text\<open>A conditional statement can be split up into multiple proofs with difference assumptions (based on the queteria)\<close>
 theorem cond_rule: "\<lbrakk>spec (\<lambda>x. p x \<and> b) S q; spec (\<lambda>x. p x \<and> \<not>b) T q\<rbrakk> \<Longrightarrow> spec p (if b then S else T) q"
   by (simp add: spec_def)
 
